switch 2

Generated/erc20shim/ERC20Shim/Common/switch_1041419350816529734_user.lean
@@ -12,12 +12,211 @@ section
 
 open Clear EVMState Ast Expr Stmt FunctionDefinition State Interpreter ExecLemmas OutOfFuelLemmas Abstraction YulNotation PrimOps ReasoningPrinciple Utilities Generated.erc20shim ERC20Shim
 
-def A_switch_1041419350816529734 (s₀ s₉ : State) : Prop := sorry
+def A_switch_1041419350816529734 (s₀ s₉ : State) : Prop :=
+  s₉.isOk ∧
+
+    (--Case 1: No initial collision
+      s₀.evm.hash_collision = false →
+      (
+      -- Case 1.1 : _24 = 0
+      (∃ slot value,
+      let s:= (Ok (sstore s₀.evm slot value) s₀.store)
+      preservesEvm s s₉) ∧
+      s₉.evm.hash_collision = false
+
+      )
+      ∨
+      ( -- Case 1.2 : Default
+        preservesEvm s₀ s₉ ∧
+        s₉.evm.hash_collision = false
+      )
+      ∨
+        -- Case 1.3 : Collision in function
+        s₉.evm.hash_collision = true
+    )
+    ∧
+    (-- Case 2: existing initial collision
+      s₀.evm.hash_collision = true →
+      s₉.evm.hash_collision = true
+    )
+
+lemma lookupAcc_preserves_eq {evm evm' : EVMState} {varstore varstore' : VarStore} :
+  preservesEvm (Ok evm varstore) (Ok evm' varstore') →
+  evm.lookupAccount evm.execution_env.code_owner = evm'.lookupAccount evm'.execution_env.code_owner := by
+  unfold lookupAccount
+  intro preserves
+  unfold preservesEvm at preserves
+  simp [Preserved_def] at preserves
+  have h1 : evm.execution_env.code_owner = evm'.execution_env.code_owner := by
+    simp [preserves.2.2.1]
+  have h2 : evm.account_map = evm'.account_map := by
+    simp [preserves]
+  rw[h1,h2]
+
+lemma updateAcc_preserved_eq {evm evm' : EVMState} {varstore varstore' : VarStore} {slot value : UInt256} {act : Account}:
+  preservesEvm (Ok evm varstore) (Ok evm' varstore') ∧
+   evm.lookupAccount evm.execution_env.code_owner = act
+  →
+  Preserved (evm.updateAccount evm.execution_env.code_owner (act.updateStorage slot value))
+            (evm'.updateAccount evm'.execution_env.code_owner (act.updateStorage slot value)) := by
+  intro h
+  obtain ⟨preserves, lookup⟩ := h
+
+  have : evm.lookupAccount evm.execution_env.code_owner = evm'.lookupAccount evm'.execution_env.code_owner := by
+    apply lookupAcc_preserves_eq preserves
+  have : evm'.lookupAccount evm'.execution_env.code_owner = act := by
+    rw[←this]
+    exact lookup
+
+  unfold preservesEvm at preserves
+  simp [Preserved_def] at preserves
+  have h1 : evm.execution_env.code_owner = evm'.execution_env.code_owner := by
+    simp [preserves.2.2.1]
+  rw[h1]
+  simp[Preserved_def]
+  unfold updateAccount
+  simp
+  obtain ⟨account, hash, exec, keccak⟩ := preserves
+  aesop
+
+lemma sstore_preserved_eq {evm evm' : EVMState} {varstore varstore' : VarStore} {slot value : UInt256} :
+  preservesEvm (Ok evm varstore) (Ok evm' varstore') →
+  preservesEvm (Ok (sstore evm slot value) varstore)
+                (Ok (sstore evm' slot value) varstore') := by
+  intro preserves
+  unfold preservesEvm
+  simp [Preserved_def]
+  have : evm.lookupAccount evm.execution_env.code_owner =
+          evm'.lookupAccount evm'.execution_env.code_owner := by
+          apply lookupAcc_preserves_eq preserves
+  have preserves_ : preservesEvm (Ok evm varstore) (Ok evm' varstore') :=
+    by exact preserves
+  unfold preservesEvm at preserves
+  simp [Preserved_def] at preserves
+  obtain ⟨account, hash, exec, keccak⟩ := preserves
+  unfold sstore
+  simp[this]
+
+  cases  h: evm'.lookupAccount evm'.execution_env.code_owner with
+  | none =>
+    simp [account, hash, exec, keccak]
+  | some act =>
+    simp[h]
+    have : Preserved (evm.updateAccount evm.execution_env.code_owner (act.updateStorage slot value))
+              (evm'.updateAccount evm'.execution_env.code_owner (act.updateStorage slot value)) := by
+              apply updateAcc_preserved_eq
+              rw[←this] at h
+              exact ⟨preserves_, h⟩
+    simp[Preserved_def] at this
+    exact this
 
 lemma switch_1041419350816529734_abs_of_concrete {s₀ s₉ : State} :
   Spec switch_1041419350816529734_concrete_of_code s₀ s₉ →
   Spec A_switch_1041419350816529734 s₀ s₉ := by
-  sorry
+  unfold switch_1041419350816529734_concrete_of_code A_switch_1041419350816529734
+
+  rcases s₀ with ⟨evm₀, varstore₀⟩ | _ | _ <;> [simp only; aesop_spec; aesop_spec]
+
+  apply spec_eq
+  clr_varstore,
+  rintro hasFuel ⟨s1, mapping,
+                  ⟨s2, update1,
+                    ⟨s3, update2, code⟩⟩⟩
+
+
+  generalize s0_all :
+  (Ok evm₀ varstore₀) = s₀ at *
+  have s0_ok : s₀.isOk := by aesop
+
+
+  by_cases _24 : s₀["_24"]!! = 0
+
+  · simp[_24] at code
+    clear update2
+
+    unfold A_mapping_index_access_mapping_address_uint256_of_address at mapping
+    clr_spec at mapping
+    unfold A_update_storage_value_offsett_uint256_to_uint256 at update1
+    clr_spec at update1
+
+    clr_varstore,
+
+    obtain ⟨s1_ok, ⟨s0s1_preserves, s0s1_state, s1_keccak, s1_no_collision⟩ | s1_collision, s0s1_collision⟩ := mapping
+
+    · -- no collision at s1 mapping
+      obtain ⟨s1_evm, ⟨s1_varstore, s1_all⟩⟩ := State_of_isOk s1_ok
+
+      obtain ⟨s2_ok, no_collision_s1, s1s2_collision⟩ := update1
+      obtain ⟨s2_evm, ⟨s2_varstore, s2_all⟩⟩ := State_of_isOk s2_ok
+
+      simp[s1_no_collision] at no_collision_s1
+
+      have s0_no_collision : s₀.evm.hash_collision = false := by aesop
+      simp[s0_no_collision]
+
+      split_ands
+      · aesop
+      · by_cases s9_collision : s₉.evm.hash_collision = false
+        · left
+          split_ands
+          · rw[←code]
+            have s1__ok : (Ok (sstore s1.evm (s1["_26"]!!) (sload s1.evm (s1["_26"]!!) + (s1["var_value"]!!)))
+                        (s1⟦"_27"↦sload s1.evm
+                                  (s1["_26"]!!)⟧⟦"_28"↦sload s1.evm
+                                (s1["_26"]!!)⟧⟦"_29"↦sload s1.evm (s1["_26"]!!) + (s1["var_value"]!!)⟧.store)).isOk := by aesop
+            have h2 : preservesEvm
+                      (Ok (sstore s1.evm (s1["_26"]!!) (sload s1.evm (s1["_26"]!!) + (s1["var_value"]!!)))
+                        (s1⟦"_27"↦sload s1.evm
+                                  (s1["_26"]!!)⟧⟦"_28"↦sload s1.evm
+                                (s1["_26"]!!)⟧⟦"_29"↦sload s1.evm (s1["_26"]!!) + (s1["var_value"]!!)⟧.store))
+                      s2 := by aesop
+            have preserves_sstore : preservesEvm
+                                    (Ok (sstore s₀.evm (s1["_26"]!!) (sload s1.evm (s1["_26"]!!) + (s1["var_value"]!!))) varstore₀)
+                                      (Ok (sstore s1.evm (s1["_26"]!!) (sload s1.evm (s1["_26"]!!) + (s1["var_value"]!!)))
+                                        (s1⟦"_27"↦sload s1.evm
+                                                  (s1["_26"]!!)⟧⟦"_28"↦sload s1.evm
+                                                (s1["_26"]!!)⟧⟦"_29"↦sload s1.evm (s1["_26"]!!) + (s1["var_value"]!!)⟧.store))
+                                                := by
+                apply sstore_preserved_eq
+                aesop
+            have s0s1_preservesEvm : preservesEvm s₀ s1 := by aesop
+            have : preservesEvm (Ok (sstore s₀.evm (s1["_26"]!!) (sload s1.evm (s1["_26"]!!) + (s1["var_value"]!!))) s₀.store) s2 := by
+              apply preservesEvm_trans s1__ok
+              · aesop
+              · aesop
+            aesop
+          · aesop
+        · aesop
+    · -- collision at s1 mapping
+      aesop
+
+  · -- Default case
+    have : 0 ≠ s₀["_24"]!! := by aesop
+    simp[this] at code
+
+    clear mapping update1 this
+
+    unfold A_update_storage_value_offsett_uint256_to_uint256 at update2
+    clr_spec at update2
+
+    obtain ⟨s3_ok, no_collision_s0, s0s3_collision⟩ := update2
+    obtain ⟨s3_evm, ⟨s3_varstore, s3_all⟩⟩ := State_of_isOk s3_ok
+
+    by_cases s0_collision : s₀.evm.hash_collision = false
+
+    · split_ands
+      · aesop
+      · simp[s0_collision]
+        by_cases s9_collision : s₉.evm.hash_collision = false
+        · left
+          split_ands
+          · rw[←code]
+            simp[s0_collision] at no_collision_s0
+            aesop
+          · aesop
+        · aesop
+      · aesop
+    · aesop
 
 end
 
